start better

Combi.v
@@ -1,303 +1,58 @@
-Set Implicit Arguments.
 Require Import Coq.Arith.Arith_base.
-
-Inductive type : Set :=
-| Iota
-| Arrow (x:type) (y:type).
 
 (* Inductive lambda {A : Set} : type -> Set :=
 | Var (t:type) (x:A) : lambda t
 | Lam (t1:type) (x:A) {t2:type} (b:lambda t2) : lambda (Arrow t1 t2)
 | App {t1 t2:type} (x:lambda (Arrow t1 t2)) (y:lambda t1) : lambda t2. *)
 
-Require Import Coq.Sets.Ensembles.
-
-(* Type of type *)
-Fixpoint tot (t:type) : Type :=
+(* Fixpoint tot t : Type :=
   match t with
   | Iota => nat
-  | Arrow x y => (tot x) -> (tot y) end.
+  | Arrow t1 t2 => (tot t1) -> (tot t2) end. *)
 
-Definition Fun {A B} (a: Ensemble A) (b: Ensemble B) : Ensemble (A -> B) :=
-  fun f => forall x, a x -> b (f x).
+Definition lt' : {_: nat | True} -> {_:nat | True} -> Prop :=
+  fun x y =>
+  match x,y with
+  | exist _ x _, exist _ y _ => lt x y end.
 
-Fixpoint comparet t : tot t -> tot t -> Prop :=
-  match t as t return tot t -> tot t -> Prop with
-  | Iota => lt
-  | Arrow t1 t2 =>
-    fun f g =>
-      let it1 := interp t1 in
-      let it2 := interp t2 in
-      (((Fun it1 it2) f /\ (Fun it1 it2) g)) /\
-      forall x, it1 x -> comparet t2 (f x) (g x)
-  end
-with interp t: Ensemble (tot t) :=
-  match t as t return Ensemble (tot t) with
-  | Iota => Full_set nat
-  | Arrow t1 t2 =>
-    fun f : tot (Arrow t1 t2) =>
-      (Fun (interp t1) (interp t2)) f /\
-      (forall v1 v2, (interp t1) v1 ->
-                     (interp t1) v2 ->
-                     comparet t1 v1 v2 -> comparet t2 (f v1) (f v2))
-  end.
+Inductive Interp : forall (T:Type) (P:T -> Prop), (sig P -> sig P -> Prop) -> Prop :=
+| Iota : Interp nat (fun _ => True) lt'
+| Arrow {t1 t2} {int1 int2} {c1 c2} (x:Interp t1 int1 c1) (y:Interp t2 int2 c2) :
+    Interp (sig int1 -> sig int2) (fun f => forall v v', c1 v v' -> c2 (f v) (f v'))
+           (fun f g => forall v, c2 (proj1_sig f v) (proj1_sig g v)).
 
-(* Prop 1 *)
-Lemma comparet_trans (t:type): forall x y z,
-    comparet t x y -> comparet t y z -> comparet t x z.
-Proof.
-  induction t.
-  - exact lt_trans.
-  - simpl; intros.
-    decompose [and] H.
-    intuition.
-    specialize H5 with x0.
-    specialize H6 with x0.
-    specialize IHt2 with (x x0) (y x0) (z x0).
-    intuition.
-Qed.
-
-Fixpoint plus (t:type) : tot t -> nat -> tot t :=
-  match t as t return tot t -> nat -> tot t with
-  | Iota => fun x k => x + k
-  | Arrow t1 t2 =>
-    fun f k =>
-      fun x => plus t2 (f x) k end.
-
-Lemma plus_arr t1 t2 : plus (Arrow t1 t2) = fun f k x => plus t2 (f x) k.
-Proof. auto. Qed.
-
-Lemma in_interp_arrow {t1 t2 v} : forall x, interp (Arrow t1 t2) v -> interp t1 x -> interp t2 (v x).
-Proof.
-  intros.
-  simpl in H.
-  destruct H as (H,_).
-  unfold Fun in H.
-  specialize H with x.
-  exact (H H0).
-Qed.
-
-Require Import Lia.
-
-Definition Plus_well_def (t:type) := forall x k, interp t x -> interp t (plus t x k).
-
-Definition Compare_compat_plus (t:type) :=
-  forall v1 v2 k,
-    interp t v1 -> interp t v2 ->
-    comparet t v1 v2 -> comparet t (plus t v1 k) (plus t v2 k).
-
-Lemma prop_2 (t:type) : Plus_well_def t /\ Compare_compat_plus t.
-Proof.
-  unfold Plus_well_def; unfold Compare_compat_plus.
-  induction t.
-  - split.
-    + intros.
-      exact (Full_intro nat (x+k)).
-    + intros; simpl. unfold comparet in H1.
-      lia.
-  - destruct IHt1 as (PWDt1,CPTt1).
-    destruct IHt2 as (PWDt2,CPTt2).
-    split.
-    + intros.
-      rewrite plus_arr; fold tot.
-      simpl.
-      split.
-      * unfold Fun.
-        intros.
-        apply PWDt2.
-        exact (in_interp_arrow x0 H H0).
-      * intros.
-        apply (CPTt2 (x v1) (x v2) k (in_interp_arrow v1 H H0) (in_interp_arrow v2 H H1)).
-        simpl in H.
-        destruct H as (_,H).
-        intuition.
-    + intros; simpl; intros.
-      fold tot.
-      split.
-      * split.
-        ** unfold Fun.
-           intros.
-           apply PWDt2.
-           exact (in_interp_arrow x H H2).
-        ** unfold Fun.
-           intros.
-           apply PWDt2.
-           exact (in_interp_arrow x H0 H2).
-      * intros.
-        apply CPTt2.
-        exact (in_interp_arrow x H H2).
-        exact (in_interp_arrow x H0 H2).
-        simpl in H1.
-        intuition.
-Qed.
-
-Lemma plus_well_def (t:type) : Plus_well_def t.
-Proof.
-  exact (proj1 (prop_2 t)).
-Qed.
-
-Lemma compare_compat_plus (t:type) : Compare_compat_plus t.
-Proof.
-  exact (proj2 (prop_2 t)).
-Qed.
-
-(* Todo: realy necessary ? *)
-Require Import Coq.Logic.FunctionalExtensionality.
-
-(* Prop 3 *)
-Lemma plus_0_neutral (t:type) : forall v, plus t v 0 = v.
-Proof.
-  intros.
-  induction t.
-  - auto.
-  - simpl.
-    fold tot.
-    extensionality x.
-    rewrite IHt2.
-    easy.
-Qed.
-
-Lemma plus_assoc (t:type) : forall v k1 k2, plus t (plus t v k1) k2 = plus t v (k1 + k2).
-Proof.
-  intros.
-  induction t.
-  - simpl. lia.
-  - simpl.
-    fold tot.
-    extensionality x.
-    rewrite IHt2.
-    easy.
-Qed.
-
-Lemma compare_plus_H (t:type) : forall v k1 k2, interp t v -> k1 < k2 -> comparet t (plus t v k1) (plus t v k2).
-Proof.
-  intros.
-  induction t.
-  - simpl. lia.
-  - simpl. fold tot.
-    simpl in H.
-    destruct H as (H1,_).
-    unfold Fun in H1.
-    repeat split.
-    * unfold Fun.
-      intros.
-      apply H1 in H.
-      apply plus_well_def; easy.
-    * unfold Fun.
-      intros.
-      apply H1 in H.
-      apply plus_well_def; easy.
-    * intros. exact (IHt2 (v x) (H1 x H)).
-Qed.
-
-Fixpoint star t: tot t :=
-  match t as t return tot t with
-  | Iota => 0
-  | Arrow t1 t2 =>
-    fun v => plus t2 (star t2) (collapse t1 v) end
-with collapse t: tot t -> nat :=
-  match t as t return tot t -> nat with
-  | Iota => fun n => n
-  | Arrow t1 t2 =>
-    fun f =>
-      collapse t2 (f (star t1)) end.
-
-Lemma prop_4 t:
-  (interp t (star t))
-  /\ (forall v v',
-         interp t v -> interp t v' -> comparet t v v' ->
-         collapse t v < collapse t v').
-Proof.
-  induction t.
-  - split.
-    + simpl. exact (Full_intro nat 0).
-    + intros; simpl; simpl in H1; assumption.
-  - destruct IHt1; destruct IHt2.
-    split.
-    + simpl.
-      fold tot.
-      split.
-      * unfold Fun.
-        intros.
-        apply plus_well_def.
-        assumption.
-      * intros.
-        specialize H0 with v1 v2.
-        apply compare_plus_H.
-        exact H1.
-        intuition.
-    + intros.
-      simpl.
-      apply H2.
-      exact (in_interp_arrow (star t1) H3 H).
-      exact (in_interp_arrow (star t1) H4 H).
-      simpl in H5.
-      intuition.
-Qed.
-
-Lemma star_well_def t : interp t (star t).
-Proof.
-  exact (proj1 (prop_4 t)).
-Qed.
-
-Lemma collapse_spec t: forall v v',
-    interp t v -> interp t v' -> comparet t v v' ->
-    collapse t v < collapse t v'.
-Proof.
-  exact (proj2 (prop_4 t)).
-Qed.
-
-(* Prop 6 *)
-Lemma collapse_star t : collapse t (star t) = 0.
-Proof.
-  induction t.
-  - auto.
-  - simpl. rewrite IHt1. rewrite plus_0_neutral. assumption.
-Qed.
-
-Lemma collapse_plus_compat t: forall v k, collapse t (plus t v k) = collapse t v + k.
-Proof.
-  intros.
-  induction t.
-  - auto.
-  - simpl.
-    exact (IHt2 (v (star t1))).
-Qed.
-
-Fixpoint le_t t : {x : (tot t) | interp t x} -> {x : (tot t) | interp t x} -> Prop :=
-  match t as t return {x : (tot t) | interp t x} -> {x : (tot t) | interp t x} -> Prop with
-  | Iota => le
-  | Arrow t1 t2 =>
-    fun f g =>
-      let it1 := interp t1 in
-      let it2 := interp t2 in
-      (((Fun it1 it2) f /\ (Fun it1 it2) g)) /\
-      forall x, In (tot t1) (interp t1) x -> le_t t2 (f x) (g x) end.
+Definition tot {T P cmp} (t:Interp T P cmp) : Type := T.
+Definition interp {T P cmp} (t:Interp T P cmp) : T -> Prop := P.
+Definition cmp {T P cmp} (t:Interp T P cmp) : sig P -> sig P -> Prop := cmp.
 
 Require Import Coq.Relations.Relation_Definitions.
 
-Lemma le_t_refl t : reflexive {x : (tot t) | interp t x} (le_t t).
+Lemma lt'_spec : forall x y, lt' x y <-> lt (proj1_sig x) (proj1_sig y).
 Proof.
-  unfold reflexive.
-  induction t.
-  - simpl. exact le_refl.
-  - intros.
-    simpl.
-    split.
-    * split.
-      ** unfold Fun.
-         intros.
-         destruct (IHt1 x0).
-         intros.
-    exact (IHt2 (x x0)).
+  intros.
+  destruct x.
+  destruct y.
+  intuition.
 Qed.
 
-Lemma le_t_sym t : antisymmetric (tot t) (le_t t).
+Lemma cmp_trans {T P C} (t:Interp T P C) : transitive (sig P) C.
 Proof.
-  unfold antisymmetric.
+  unfold transitive.
+  intros.
   induction t.
-  - simpl. exact le_antisym.
+  - destruct x. destruct y. destruct z.
+    simpl; simpl in H; simpl in H0.
+    exact (lt_trans x x0 x1 H H0).
   - intros.
-    simpl in H.
-    simpl in H0.
-    extensionality z.
+    apply IHt2 with (y := (proj1_sig y v)).
+    intuition. intuition.
+Qed.
+
+Fixpoint plus {T P C} (t:Interp T P C) : sig P -> nat -> sig P :=
+  match t with
+  | Iota => fun x k => exist (fun _ => True) (proj1_sig x + k) I
+  | Arrow x y =>
+    fun f k =>
+      let f' := fun v => plus y (proj1_sig f v) k in
+      sexist (fun f => forall v v', (cmp x) v v' -> cmp y (f v) (f v'))
+  end.
